moved StrongSubset reasoning to separate file

examples/ghc/theories/Var.v
@@ -184,6 +184,8 @@ Proof.
 Qed.
 
 
+
+
 (** ** [almostEqual] *)
 
 (* Two [Var]s are almostEqual if they differ only in 
@@ -228,6 +230,18 @@ Proof.
   econstructor.
 Qed.
 
+Instance Equivalence_ae : Equivalence almostEqual.
+Proof.
+  split. 
+  - unfold Reflexive.
+    apply almostEqual_refl.
+  - unfold Symmetric.
+    eauto using almostEqual_sym.
+  - unfold Transitive.
+    intros x y z h1 h2.
+    eapply almostEqual_trans; eauto.
+Defined.
+
 Lemma almostEqual_eq :
   forall v1 v2, 
     almostEqual v1 v2 -> (v1 == v2).
@@ -235,6 +249,29 @@ Proof.
   intros v1 v2 H.
   inversion H; unfold_zeze; simpl; apply N.eqb_refl.
 Qed.
+
+Instance eq_m :
+  Proper ((fun (x y:Var) => x == y) ==> (fun x y => x == y) ==> Logic.eq) (fun (x y : Var) => (x == y)).
+Proof.
+  unfold_zeze.
+  move=> x1 y1 E1 x2 y2 E2.
+  apply N.eqb_eq in E1.
+  apply N.eqb_eq in E2.
+  rewrite E1. rewrite E2.
+  eauto.
+Qed.
+
+Instance almostEqual_eq_m :
+  Proper (almostEqual ==> almostEqual ==> Logic.eq) (fun (x y : Var) => (x == y)).
+Proof.
+  move=> x1 y1 E1 x2 y2 E2.
+  apply almostEqual_eq in E1.
+  apply almostEqual_eq in E2.
+  rewrite -> E1.
+  rewrite -> E2.
+  auto.
+Qed.
+
 
 (** ** [isJoinId] etc. *)
 
@@ -337,3 +374,17 @@ Proof.
   auto.
 Qed.
 Hint Resolve RespectsVar_isLocalVar.
+
+
+Definition RespectsAEVar (f :Var -> bool) :=
+    Proper ((fun x0 y : Var => almostEqual x0 y) ==> Logic.eq) f.
+Lemma RespectsAEVar_isLocalVar : RespectsAEVar isLocalVar.
+Proof.
+  move=> v1 v2.
+  move=> h.
+  apply almostEqual_eq in h.
+  rewrite -> varUnique_iff  in h.
+  unfold isLocalVar. unfold isGlobalId. rewrite h.
+  auto.
+Qed.
+Hint Resolve RespectsAEVar_isLocalVar.
