examples/ghc/manual/IntMap.v
@@ -162,6 +162,7 @@ Section IntMap.
 
 End IntMap.
 
+
 (** These should be in [containers]. *)
 
 Lemma list_KeyIn : forall {A B} `{Base.EqLaws A} `{Base.EqLaws B}
