examples/ghc/theories/CoreSubst.v
@@ -25,6 +25,7 @@ Require Import Proofs.CoreInduct.
 Require Import Proofs.Core.
 Require Import Proofs.VarSet.
 Require Import Proofs.VarSetFSet.
+Require Import Proofs.VarSetStrong.
 Require Import Proofs.VarEnv.
 Require Import Proofs.Var.
 Require Import Proofs.ScopeInvariant.
@@ -509,14 +510,14 @@ Ltac destruct_SubstExtends :=
     | [ H : SubstExtends ?s1 ?vs ?s2 ?vs1 |- _ ] => 
       try (is_var s1 ; destruct s1);
       try (is_var s2 ; destruct s2);
-      unfold SubstExtends in H; repeat (destruct_one_pair)
+      unfold SubstExtends in H;  unfold StrongEquivalence in *; repeat (destruct_one_pair)
     end.
 
 
 (* Prove goals about lookupVarSet, given StrongSubset assumptions *)
 Ltac lookup_StrongSubset :=
     match goal with 
-      [ h1 : StrongSubset (extendVarSetList ?i3 ?vars1) ?i,
+      [ h1 : (extendVarSetList ?i3 ?vars1) {<=} ?i,
         h2 : forall v:Var, is_true (Foldable.elem v ?vars1) -> lookupVarSet ?i3 v = None,
         m  : lookupVarSet ?i ?v  = ?r |- 
              lookupVarSet ?i3 ?v = ?r ] =>
@@ -542,7 +543,6 @@ Proof.
   apply freshList_nil.
   eapply StrongSubset_refl.
   eapply StrongSubset_refl.
-(*   eapply strongSubset_implies_subset. *)
   eapply StrongSubset_minusDom_left.
   intros var.
   destruct lookupVarEnv eqn:LU; try tauto.
@@ -634,43 +634,43 @@ Proof.
        apply almostEqual_refl.
        eapply Eq_trans; first rewrite Eq_sym; eassumption.
      +  clear VEmf H5.
-        rewrite lookupVarSet_minusDom_1 in H13; try done.
-       rewrite ELEM2 in VEim.
-       case InV2: (Foldable.elem var vars2); hs_simpl.
-       ++ move:(lookupVarSet_extendVarSetList_self_exists_LastIn 
+        rewrite -> lookupVarSet_minusDom_1 in H13; try done.
+        rewrite ELEM2 in VEim.
+        case InV2: (Foldable.elem var vars2); hs_simpl.
+        ++ move:(lookupVarSet_extendVarSetList_self_exists_LastIn 
                    (extendVarSetList (getInScopeVars init_scope) vars1) InV2) => [v1 [-> q1 r1]].
-          move:(lookupVarSet_extendVarSetList_self_exists_LastIn 
-                  (getInScopeVars mid_scope) InV2) => [v2 [p2 q2 r2]].
-          rewrite p2 in H6.
-          destruct (lookupVarSet (getInScopeVars fin_scope) var) eqn:InF; try done.
-          eapply LastIn_inj in r2; try eapply r1.
-          subst. auto.
-          eapply Eq_trans; first rewrite Eq_sym; eassumption.
-       ++ have InV2': ~~ Foldable.elem var vars2 by rewrite InV2.
-          rewrite lookupVarSet_extendVarSetList_false //.
-          rewrite lookupVarSet_extendVarSetList_false // in H6.
-          case InV1: (Foldable.elem var vars1); hs_simpl.
-          ** move:(lookupVarSet_extendVarSetList_self_exists_LastIn 
-                   (getInScopeVars init_scope) InV1) => [v1 [p1 q1 r1]].
-            rewrite p1.
-            rewrite p1 in H13.
-            case InM1: (lookupVarSet (getInScopeVars mid_scope) var) => [b|]; 
-            rewrite InM1 in H13; try done.
-            rewrite InM1 in H6.
-            case InF1: (lookupVarSet (getInScopeVars fin_scope) var) => [cc|]; 
-            rewrite InF1 in H6; try done.
-            eapply almostEqual_trans; eauto.
-          ** have InV1': ~~ Foldable.elem var vars1 by rewrite InV1.
-          rewrite lookupVarSet_extendVarSetList_false //.
-          rewrite lookupVarSet_extendVarSetList_false // in H13.
-          case InI1: (lookupVarSet (getInScopeVars init_scope) var) => [a|] //.
-          rewrite InI1 in H13.
-          case InM1: (lookupVarSet (getInScopeVars mid_scope) var) => [b|] //;
-             rewrite InM1 // in H13.
-          rewrite InM1 in H6.         
-          case InF1: (lookupVarSet (getInScopeVars fin_scope) var) => [cc|] //;
-             rewrite InF1 // in H6.
-          eapply almostEqual_trans; eauto.          
+           move:(lookupVarSet_extendVarSetList_self_exists_LastIn 
+                   (getInScopeVars mid_scope) InV2) => [v2 [p2 q2 r2]].
+           rewrite p2 in H6.
+           destruct (lookupVarSet (getInScopeVars fin_scope) var) eqn:InF; try done.
+           eapply LastIn_inj in r2; try eapply r1.
+           subst. auto.
+           eapply Eq_trans; first rewrite Eq_sym; eassumption.
+        ++ have InV2': ~~ Foldable.elem var vars2 by rewrite InV2.
+           rewrite lookupVarSet_extendVarSetList_false //.
+           rewrite lookupVarSet_extendVarSetList_false // in H6.
+           case InV1: (Foldable.elem var vars1); hs_simpl.
+           ** move:(lookupVarSet_extendVarSetList_self_exists_LastIn 
+                      (getInScopeVars init_scope) InV1) => [v1 [p1 q1 r1]].
+              rewrite p1.
+              rewrite p1 in H13.
+              case InM1: (lookupVarSet (getInScopeVars mid_scope) var) => [b|]; 
+                                                                           rewrite InM1 in H13; try done.
+              rewrite InM1 in H6.
+              case InF1: (lookupVarSet (getInScopeVars fin_scope) var) => [cc|]; 
+                                                                           rewrite InF1 in H6; try done.
+              eapply almostEqual_trans; eauto.
+           ** have InV1': ~~ Foldable.elem var vars1 by rewrite InV1.
+              rewrite lookupVarSet_extendVarSetList_false //.
+              rewrite lookupVarSet_extendVarSetList_false // in H13.
+              case InI1: (lookupVarSet (getInScopeVars init_scope) var) => [a|] //.
+              rewrite InI1 in H13.
+              case InM1: (lookupVarSet (getInScopeVars mid_scope) var) => [b|] //;
+                                                                              rewrite InM1 // in H13.
+              rewrite InM1 in H6.         
+              case InF1: (lookupVarSet (getInScopeVars fin_scope) var) => [cc|] //;
+                                                                               rewrite InF1 // in H6.
+              eapply almostEqual_trans; eauto.          
 Qed.
 
 Lemma Subset_VarEnvExtends : forall old_env vars new_env vars' vs1 vs2,
