examples/ghc/theories/VarSet.v
@@ -20,13 +20,14 @@ Require Import Id.
 Require Import Core.
 Require UniqFM.
 
+Require Import Proofs.Base.
 Require Import Proofs.Axioms.
 Require Import Proofs.ContainerAxioms.
 Require Import Proofs.GhcTactics.
 Require Import Proofs.Unique.
 Require Import Proofs.Var.
 Require Import Proofs.VarSetFSet.
-Require Import Proofs.Base.
+
 
 Open Scope Z_scope.
 
@@ -2125,91 +2126,6 @@ Proof.
   unfold UniqFM.delFromUFM; simpl; auto.
 Qed.
 
-(** ** [StrongSubset] *)
-
-
-(* A strong subset doesn't just have a subset of the uniques, but 
-     also requires that the variables in common be almostEqual. *)
-Definition StrongSubset (vs1 : VarSet) (vs2: VarSet) := 
-  forall var, match lookupVarSet vs1 var with 
-           | Some v =>  match lookupVarSet vs2 var with
-                          | Some v' => almostEqual v v'
-                          | None => False
-                       end
-           | None => True 
-         end.
-
-
-Notation "s1 {<=} s2" := (StrongSubset s1 s2) (at level 70, no associativity).
-Notation "s1 {=} s2" := (StrongSubset s1 s2 /\ StrongSubset s2 s1) (at level 70, no associativity).
-
-
-Lemma StrongSubset_refl : forall vs, 
-    StrongSubset vs vs.
-Proof.
-  unfold StrongSubset.
-  move=> vs var.
-  elim h: (lookupVarSet vs var) => //.
-  eapply almostEqual_refl.
-Qed.
-
-Instance StrongSubset_Reflexive : Reflexive StrongSubset := StrongSubset_refl.
-
-Lemma StrongSubset_trans : forall vs1 vs2 vs3, 
-    StrongSubset vs1 vs2 -> StrongSubset vs2 vs3 -> StrongSubset vs1 vs3.
-Proof.
-  move => vs1 vs2 vs3 h1 h2 var.
-  specialize (h1 var).
-  specialize (h2 var).
-  move: h1 h2.
-  elim p1: (lookupVarSet vs1 var) => //;
-  elim p2: (lookupVarSet vs2 var) => //;
-  elim p3: (lookupVarSet vs3 var) => //.
-  eapply almostEqual_trans.
-Qed.
-
-
-Instance StrongSubset_Transitive : Transitive StrongSubset := StrongSubset_trans.
-
-
-Lemma strongSubset_implies_subset :
-  forall vs1 vs2 , 
-    StrongSubset vs1 vs2 -> vs1 [<=] vs2.
-Proof. 
-  intros vs1 vs2.
-  unfold StrongSubset, Subset.
-  intros SS var IN.
-  unfold In in *.
-  specialize (SS var). 
-  destruct (lookupVarSet vs1 var) eqn:VS1;
-  destruct (lookupVarSet vs2 var) eqn:VS2; try contradiction.
-  - apply lookupVarSet_elemVarSet in VS2.   
-    auto.
-  - apply elemVarSet_lookupVarSet in IN. destruct IN.
-    rewrite VS1 in H. discriminate.
-  - apply elemVarSet_lookupVarSet in IN. destruct IN.
-    rewrite VS1 in H. discriminate.
-Qed.
-
-
-
-Lemma StrongSubset_extend_fresh :
-  forall vs v,
-  lookupVarSet vs v = None ->
-  StrongSubset vs (extendVarSet vs v).
-Proof.
-  intros.
-  unfold StrongSubset.
-  intros var.
-  destruct (var == v) eqn:EQV.
-  rewrite -> lookupVarSet_eq with (v2 := v); auto.
-  rewrite H. auto.
-  destruct (lookupVarSet vs var) eqn:Lvar; auto.
-  rewrite lookupVarSet_extendVarSet_neq.
-  rewrite Lvar.
-  apply almostEqual_refl.
-  unfold CoreBndr in *. intro h. rewrite Base.Eq_sym in h. rewrite h in EQV. discriminate.
-Qed.
 
 Lemma elemNegbDisjoint : forall vs vs2, 
     disjointVarSet vs (mkVarSet vs2) ->
@@ -2230,74 +2146,6 @@ Qed.
 
 
 
-Lemma StrongSubset_extendList_fresh :
-  forall vs vs2,
-  disjointVarSet vs (mkVarSet vs2)  ->
-  StrongSubset vs (extendVarSetList vs vs2).
-Proof.
-  intros.
-  unfold StrongSubset.
-  intros v.
-  destruct_match; try trivial.
-  case in2: (Foldable.elem v vs2).  
-  * eapply elemNegbDisjoint in in2; eauto.
-    eapply lookupVarSet_elemVarSet in Heq; eauto. 
-    erewrite Heq in in2. done.
-  * rewrite lookupVarSet_extendVarSetList_false; try done.
-    rewrite Heq.
-    eapply almostEqual_refl.
-    rewrite in2. done.
-Qed.
-
-
-Lemma StrongSubset_extend_ae :
-  forall vs1 vs2 v1 v2,
-  StrongSubset vs1 vs2 ->
-  almostEqual v1 v2 ->
-  StrongSubset (extendVarSet vs1 v1) (extendVarSet vs2 v2).
-Proof.
-  intros.
-  unfold StrongSubset in *.
-  intro var.
-  destruct (v1 == var) eqn:EQv.
-  rewrite lookupVarSet_extendVarSet_eq; auto.  
-  rewrite lookupVarSet_extendVarSet_eq.
-  assumption.
-  apply almostEqual_eq in H0. eapply Eq_trans; try eassumption; try symmetry; assumption.
-  rewrite lookupVarSet_extendVarSet_neq; auto.
-  rewrite lookupVarSet_extendVarSet_neq; auto.
-  eapply H.
-  rewrite <- not_true_iff_false in EQv. contradict EQv.
-  apply almostEqual_eq in H0. eapply Eq_trans; try eassumption; try symmetry; assumption.
-  rewrite not_true_iff_false. assumption.
-Qed.
-
-
-Lemma StrongSubset_extend :
-  forall vs1 vs2 v,
-  StrongSubset vs1 vs2 ->
-  StrongSubset (extendVarSet vs1 v) (extendVarSet vs2 v).
-Proof.
-  intros.
-  apply StrongSubset_extend_ae.
-  * assumption.
-  * apply almostEqual_refl.
-Qed.
-
-Lemma StrongSubset_extendVarSetList_ae :
-  forall l1 l2 vs1 vs2,
-  Forall2 almostEqual l1 l2 ->
-  StrongSubset vs1 vs2 ->
-  StrongSubset (extendVarSetList vs1 l1) (extendVarSetList vs2 l2).
-Proof.
-  intros.
-  revert vs1 vs2 H0. induction H; intros.
-  * apply H0.
-  * rewrite extendVarSetList_cons.
-    apply IHForall2.
-    apply StrongSubset_extend_ae; assumption.
-Qed.
-
 Lemma Forall2_diag:
   forall a P (xs: list a),
   Forall2 P xs xs <-> Forall (fun x => P x x) xs.
@@ -2308,16 +2156,6 @@ Proof.
   * split; intro H; constructor; inversion H; intuition.
 Qed.
 
-Lemma StrongSubset_extendVarSetList :
-  forall l vs1 vs2,
-  StrongSubset vs1 vs2 ->
-  StrongSubset (extendVarSetList vs1 l) (extendVarSetList vs2 l).
-Proof.
-  intros.
-  apply StrongSubset_extendVarSetList_ae; only 2: assumption.
-  apply Forall2_diag.
-  rewrite Forall_forall. intros. apply almostEqual_refl.
-Qed.
 
 Lemma lookupVarSet_delVarSet_None:
   forall v vs, lookupVarSet (delVarSet vs v) v = None.
@@ -2333,251 +2171,6 @@ Proof.
   destruct getUniqSet'.
   simpl.
   apply delete_eq.
-Qed.
-
-Lemma StrongSubset_delVarSet :
-  forall vs1 vs2 v,
-  StrongSubset vs1 vs2 ->
-  StrongSubset (delVarSet vs1 v) (delVarSet vs2 v).
-Proof.
-  intros.
-  unfold StrongSubset in *.
-  intro var.
-  specialize (H var).
-  destruct (v == var) eqn:EQv.
-  - rewrite Base.Eq_sym in EQv.
-    erewrite lookupVarSet_eq;
-      [|eassumption].
-    rewrite lookupVarSet_delVarSet_None.
-    trivial.
-  - rewrite lookupVarSet_delVarSet_neq;
-      [|rewrite EQv; auto].
-    destruct (lookupVarSet vs1 var) eqn:Hl; auto.
-    rewrite lookupVarSet_delVarSet_neq;
-      [|rewrite EQv; auto].
-    auto.
-Qed.
-
-Lemma StrongSubset_delete_fresh :
-  forall vs v,
-  lookupVarSet vs v = None ->
-  StrongSubset vs (delVarSet vs v).
-Proof.
-  intros.
-  unfold StrongSubset in *.
-  intro var.
-  destruct (v == var) eqn:EQv.
-  - rewrite Base.Eq_sym in EQv.
-    erewrite lookupVarSet_eq;
-      [|eassumption].
-    rewrite H.
-    trivial.
-  - rewrite lookupVarSet_delVarSet_neq;
-      [|rewrite EQv; auto].
-    destruct (lookupVarSet vs var) eqn:Hl; auto.
-    apply almostEqual_refl.
-Qed.
-
-Lemma StrongSubset_delVarSetList:
-  forall vs1 vs2 vs,
-  StrongSubset vs1 vs2 ->
-  StrongSubset (delVarSetList vs1 vs) (delVarSetList vs2 vs).
-Proof.
-  intros vs1 vs2 vs.
-  generalize dependent vs2.
-  generalize dependent vs1.
-  induction vs;
-    intros vs1 vs2 H; hs_simpl;
-      [assumption|].
-  eapply StrongSubset_delVarSet in H.
-  eauto.
-Qed.
-
-(* Respects_StrongSubset *)
-
-Definition Respects_StrongSubset (P : VarSet -> Prop) : Prop :=
-  forall (vs1 vs2 : VarSet),
-  StrongSubset vs1 vs2 ->
-  P vs1 -> P vs2.
-Existing Class Respects_StrongSubset.
-
-Require Import Coq.Classes.Morphisms.
-Global Instance Respects_StrongSubset_iff_morphism:
-  Proper (pointwise_relation VarSet iff ==> iff) Respects_StrongSubset.
-Proof.
-  intros ???.
-  split; intros ?????;
-  unfold pointwise_relation in H;
-  firstorder.
-Qed.
-
-Lemma Respects_StrongSubset_const:
-  forall P, Respects_StrongSubset (fun _ => P).
-Proof. intros ?????. assumption. Qed.
-
-Lemma Respects_StrongSubset_and:
-  forall P Q,
-    Respects_StrongSubset P ->
-    Respects_StrongSubset Q ->
-    Respects_StrongSubset (fun x => P x /\ Q x).
-Proof.
-  unfold Respects_StrongSubset in *.
-  intros ????????.
-  firstorder.
-Qed.
-
-Lemma Respects_StrongSubset_andb:
-  forall (P Q : VarSet -> bool),
-    Respects_StrongSubset (fun x => P x = true) ->
-    Respects_StrongSubset (fun x => Q x = true) ->
-    Respects_StrongSubset (fun x => P x && Q x = true).
-Proof.
-  unfold Respects_StrongSubset in *.
-  intros ????????.
-  simpl_bool.
-  firstorder.
-Qed.
-
-
-Lemma Respects_StrongSubset_forall:
-  forall a (xs : list a) P,
-    Forall (fun x => Respects_StrongSubset (fun vs => P vs x)) xs ->
-    Respects_StrongSubset (fun vs => Forall (P vs) xs).
-Proof.
-  unfold Respects_StrongSubset in *.
-  intros.
-  rewrite -> Forall_forall in *.
-  firstorder.
-Qed.
-
-Lemma Respects_StrongSubset_forallb:
-  forall a (xs : list a) P,
-    Forall (fun x => Respects_StrongSubset (fun vs => P vs x = true)) xs ->
-    Respects_StrongSubset (fun vs => forallb (P vs) xs = true).
-Proof.
-  unfold Respects_StrongSubset in *.
-  intros.
-  rewrite -> forallb_forall in *.
-  rewrite -> Forall_forall in *.
-  firstorder.
-Qed.
-
-
-Lemma Respects_StrongSubset_elemVarSet:
-  forall v,
-  Respects_StrongSubset (fun vs => elemVarSet v vs = true).
-Proof.
-  intros ????.
-  simpl_bool; intuition.
-  apply strongSubset_implies_subset in H.
-  set_b_iff; fsetdec.
-Qed.
-
-Lemma Respects_StrongSubset_delVarSet:
-  forall v P,
-  Respects_StrongSubset (fun vs : VarSet => P vs) ->
-  Respects_StrongSubset (fun vs : VarSet => P (delVarSet vs v)).
-Proof.
-  intros v P H vs1 vs2 Hs Hvs1.
-  apply StrongSubset_delVarSet with (v:=v) in Hs.
-  unfold Respects_StrongSubset in H.  
-  apply H in Hs; auto.
-Qed.
-
-Lemma Respects_StrongSubset_delVarSetList:
-  forall vs2 P,
-  Respects_StrongSubset (fun vs : VarSet => P vs) ->
-  Respects_StrongSubset (fun vs : VarSet => P (delVarSetList vs vs2)).
-Proof.
-  intros vs2 P H vs vs' Hs Hvs2.
-  apply StrongSubset_delVarSetList with (vs:=vs2) in Hs.
-  unfold Respects_StrongSubset in H.  
-  apply H in Hs; auto.
-Qed.
-
-
-Lemma Respects_StrongSubset_extendVarSet:
-  forall v P,
-  Respects_StrongSubset (fun vs : VarSet => P vs) ->
-  Respects_StrongSubset (fun vs : VarSet => P (extendVarSet vs v)).
-Proof.
-  intros v P H vs vs' Hs Hvs.
-  apply StrongSubset_extend with (v:=v) in Hs.
-  unfold Respects_StrongSubset in H.
-  apply H in Hs; auto.
-Qed.
-
-
-Lemma Respects_StrongSubset_extendVarSetList:
-  forall vs' P,
-  Respects_StrongSubset (fun vs : VarSet => P vs) ->
-  Respects_StrongSubset (fun vs : VarSet => P (extendVarSetList vs vs')).
-Proof.
-  intros vs P H vs1 vs2 Hs Hvs1.
-  eapply StrongSubset_extendVarSetList with (l:=vs) in Hs.
-  unfold Respects_StrongSubset in H.
-  apply H in Hs; auto.
-Qed. 
-
-Lemma StrongSubset_filterVarSet: 
-  forall f1 f2 vs,
-    RespectsVar f1 -> RespectsVar f2 ->
-  (forall v, f1 v = true  -> f2 v = true) ->
-  filterVarSet f1 vs {<=} filterVarSet f2 vs.
-Proof.
-  intros.
-  unfold StrongSubset.
-  intros var.
-  destruct (f1 var) eqn:Heq1.
-  - rewrite lookupVarSet_filterVarSet_true; auto.
-    destruct (lookupVarSet vs var) eqn:Hl; [|trivial].
-    rewrite lookupVarSet_filterVarSet_true; auto.
-    rewrite Hl.
-    apply almostEqual_refl.
-  - rewrite lookupVarSet_filterVarSet_false; auto.
-Qed.
-
-(* Is this weakening? *)
-Lemma weaken:
-  forall {P : VarSet -> Prop} {R : Respects_StrongSubset P},
-  forall {vs1} {vs2},
-  StrongSubset vs1 vs2 ->
-  P vs1 -> P vs2.
-Proof. intros. unfold Respects_StrongSubset in R. eapply R; eassumption. Qed.
-
-Lemma weakenb:
-  forall {P : VarSet -> bool} {R : Respects_StrongSubset (fun x => P x )},
-  forall {vs1} {vs2},
-  StrongSubset vs1 vs2 ->
-  P vs1  -> P vs2 .
-Proof. intros. unfold Respects_StrongSubset in R. eapply R; eassumption. Qed.
-
-Lemma Respects_StrongSubset_extendVarSet_ae:
-  forall {P : VarSet -> Prop} {R : Respects_StrongSubset P},
-  forall vs v1 v2,
-  almostEqual v1 v2 ->
-  P (extendVarSet vs v1) <-> P (extendVarSet vs v2).
-Proof.
-  intros.
-  split; apply R; (apply StrongSubset_extend_ae;
-    [ reflexivity | assumption + (apply almostEqual_sym; assumption) ]).
-Qed.
-
-
-Lemma Respects_StrongSubset_extendVarSetList_ae:
-  forall {P : VarSet -> Prop} {R : Respects_StrongSubset P},
-  forall vs vs1 vs2,
-  Forall2 almostEqual vs1 vs2 ->
-  P (extendVarSetList vs vs1) <-> P (extendVarSetList vs vs2).
-Proof.
-  split; apply R; apply StrongSubset_extendVarSetList_ae.
-  * assumption.
-  * reflexivity.
-  * clear -H.
-    induction H; constructor.
-    + apply almostEqual_sym; assumption.
-    + assumption.
-  * reflexivity.
 Qed.
 
 
@@ -2637,26 +2230,6 @@ Proof.
     rewrite <- freshList_cons in *. tauto.
 Qed.
     
-Lemma StrongSubset_extendVarSet_fresh : 
-  forall vs var, lookupVarSet vs var = None ->
-            StrongSubset vs (extendVarSet vs var).
-Proof.
-  apply StrongSubset_extend_fresh.
-Qed.
-
-Lemma StrongSubset_extendVarSetList_fresh : 
-  forall vs vars, freshList vars vs ->
-             StrongSubset vs (extendVarSetList vs vars).
-Proof.
-  intros.
-  apply StrongSubset_extendList_fresh.
-  apply disjointVarSet_mkVarSet.
-  induction vars; auto.
-  apply freshList_cons in H as [H1 H2].
-  apply Forall_cons; auto.
-  apply lookupVarSet_None_elemVarSet.
-  assumption.
-Qed.
 
 
 Lemma elemVarSet_unitVarSet_is_eq :
